src/tosmt/term.fsi
@@ -44,8 +44,8 @@ type term' =
   | PP         of term * term
   | App        of string * list<term>
   | Not        of term
-  | And        of term * term
-  | Or         of term * term
+  | And        of list<term>
+  | Or         of list<term>
   | Imp        of term * term
   | Iff        of term * term
   | Eq         of term * term
@@ -67,8 +67,10 @@ type term' =
   | ConstArray of string * sort * term 
   | Cases      of list<term>
 and pat = term
-and term = {tm:term'}
+and term = {tm:term'; as_str:string; freevars:Syntax.memo<list<var>>}
 and var = (string * sort)
+
+val free_variables: term -> list<(string * sort)>
 
 val mkTrue : term
 val mkFalse : term
@@ -118,10 +120,10 @@ type decl =
   | Push
   | Pop
   | CheckSat
-type decls = list<decl>
+type decls_t = list<decl>
 
-val constructor_to_decl: constructor_t -> decls
-val termToSmt: binders -> term -> string
+val constructor_to_decl: constructor_t -> decls_t
+val termToSmt: term -> string
 val declToSmt: string -> decl -> string
 
 val mk_Kind_type : term
